coq/02-closure/NullRingCloses.v
@@ -1,0 +1,139 @@
+(**
+  The Null Ring closure invariant.
+
+  Readable forms are not asserted to be textually identical. They are related
+  by the same explicitly defined XOR closure result.
+*)
+
+From Coq Require Import NArith List Bool Lia.
+Import ListNotations.
+
+Open Scope N_scope.
+
+Definition xor_reduce (xs : list N) : N :=
+  fold_right N.lxor 0 xs.
+
+Definition edge_witness (edge : N * N) : N :=
+  N.lxor (fst edge) (snd edge).
+
+Definition edge_witnesses (edges : list (N * N)) : list N :=
+  map edge_witness edges.
+
+Definition byte_ring_edges : list (N * N) :=
+  [(0, 32); (32, 127); (127, 255); (255, 0)].
+
+Definition byte_ring_witnesses : list N :=
+  edge_witnesses byte_ring_edges.
+
+Theorem xor_self_cancels :
+  forall x, N.lxor x x = 0.
+Proof. apply N.lxor_nilpotent. Qed.
+
+Theorem byte_ring_witness_values :
+  byte_ring_witnesses = [32; 95; 128; 255].
+Proof. vm_compute; reflexivity. Qed.
+
+Theorem byte_ring_closes_to_null :
+  xor_reduce byte_ring_witnesses = 0.
+Proof. vm_compute; reflexivity. Qed.
+
+Lemma xor_reduce_app :
+  forall xs ys,
+    xor_reduce (xs ++ ys) = N.lxor (xor_reduce xs) (xor_reduce ys).
+Proof.
+  induction xs as [|x xs IH]; intro ys.
+  - reflexivity.
+  - simpl. rewrite IH. rewrite N.lxor_assoc. reflexivity.
+Qed.
+
+Theorem duplicated_boundary_closes :
+  forall xs, xor_reduce (xs ++ xs) = 0.
+Proof.
+  intro xs.
+  rewrite xor_reduce_app.
+  apply N.lxor_nilpotent.
+Qed.
+
+Fixpoint adjacent_edges (start previous : N) (rest : list N)
+  : list (N * N) :=
+  match rest with
+  | [] => [(previous, start)]
+  | x :: xs => (previous, x) :: adjacent_edges start x xs
+  end.
+
+Definition closed_path_edges (vertices : list N) : list (N * N) :=
+  match vertices with
+  | [] => []
+  | x :: xs => adjacent_edges x x xs
+  end.
+
+Lemma adjacent_edge_witnesses_telescope :
+  forall start previous rest,
+    xor_reduce (edge_witnesses (adjacent_edges start previous rest)) =
+    N.lxor previous start.
+Proof.
+  intros start previous rest.
+  revert previous.
+  induction rest as [|x xs IH]; intro previous.
+  - simpl. rewrite N.lxor_0_r. reflexivity.
+  - simpl. rewrite IH.
+    unfold edge_witness; simpl.
+    rewrite N.lxor_assoc.
+    rewrite <- (N.lxor_assoc x x start).
+    rewrite N.lxor_nilpotent.
+    rewrite N.lxor_0_l.
+    reflexivity.
+Qed.
+
+Theorem every_closed_path_closes :
+  forall vertices,
+    xor_reduce (edge_witnesses (closed_path_edges vertices)) = 0.
+Proof.
+  intros [|start rest].
+  - reflexivity.
+  - unfold closed_path_edges.
+    rewrite adjacent_edge_witnesses_telescope.
+    apply N.lxor_nilpotent.
+Qed.
+
+Theorem concrete_closed_path_matches_byte_ring :
+  closed_path_edges [0; 32; 127; 255] = byte_ring_edges.
+Proof. reflexivity. Qed.
+
+Theorem concrete_closed_path_closes :
+  xor_reduce (edge_witnesses (closed_path_edges [0; 32; 127; 255])) = 0.
+Proof. vm_compute; reflexivity. Qed.
+
+Definition address256 (x : N) : Prop := x < N.pow 2 256.
+
+Theorem address256_self_cancels :
+  forall address,
+    address256 address ->
+    N.lxor address address = 0.
+Proof.
+  intros address _.
+  apply N.lxor_nilpotent.
+Qed.
+
+Inductive NullPresentation : Type :=
+| FoldedNull
+| UnfoldedByteRing
+| FullNotationNull.
+
+Definition null_closure_value (presentation : NullPresentation) : N :=
+  match presentation with
+  | FoldedNull => N.lxor 0 0
+  | UnfoldedByteRing => xor_reduce byte_ring_witnesses
+  | FullNotationNull => N.lxor (N.pow 2 255) (N.pow 2 255)
+  end.
+
+Theorem all_null_presentations_share_closure :
+  forall presentation, null_closure_value presentation = 0.
+Proof. destruct presentation; vm_compute; reflexivity. Qed.
+
+Theorem folded_unfolded_full_closure_equivalent :
+  null_closure_value FoldedNull =
+  null_closure_value UnfoldedByteRing /\
+  null_closure_value UnfoldedByteRing =
+  null_closure_value FullNotationNull.
+Proof. vm_compute; split; reflexivity. Qed.
